notations.lean
@@ -33,6 +33,13 @@ infix `||` := has_or.or
 -- use • as hole
 notation `•` := termctx.hole
 
+-- history items
+@[reducible]
+def nop := historyitem.nop
+
+@[reducible]
+def call := historyitem.call
+
 -- simple coercions
 instance value_to_term : has_coe value term := ⟨term.value⟩
 instance var_to_term : has_coe var term := ⟨term.var⟩
@@ -209,12 +216,9 @@ instance : has_coe_to_fun propctx := ⟨λ _, term → prop, propctx.apply⟩
 
 -- call history to prop coercion
 
-def calls_to_prop: list call → prop
-| list.nil := value.true
-| (⟨f, x, R, S, e, σ, vₓ, v⟩ :: rest) :=
-    prop.call (value.func f x R S e σ) vₓ &&
-    prop.post (value.func f x R S e σ) vₓ &&
-    (term.app (value.func f x R S e σ) vₓ ≡ v) &&
-    calls_to_prop rest
+def calls_to_prop: callhistory → prop
+| list.nil                                  := value.true
+| (historyitem.nop :: rest)                 := calls_to_prop rest
+| (historyitem.call f x R S e σ vₓ :: rest) := prop.call (value.func f x R S e σ) vₓ && calls_to_prop rest
 
-instance call_to_prop: has_coe (list call) prop := ⟨calls_to_prop⟩
+instance call_to_prop: has_coe callhistory prop := ⟨calls_to_prop⟩
