vcgen.lean
@@ -22,9 +22,8 @@ notation P `⊢` e `:` Q : 10 := exp.vcgen P e Q
 
 | func {P: prop} {f x: var} {R S: spec} {e₁ e₂: exp} {Q₁ Q₂: propctx}:
     f ∉ FV P →
-    x ∉ FV P →
-    FV R.to_prop ⊆ FV P →
-    FV S.to_prop ⊆ FV P →
+    FV R.to_prop ⊆ FV P ∪ { f, x } →
+    FV S.to_prop ⊆ FV P ∪ { f, x } →
     (P && spec.func f x R S && R ⊢ e₁ : Q₁) →
     (P && spec.func f x R S ⊢ e₂ : Q₂) →
     ⟪prop.implies (P && spec.func f x R S && R && Q₁ (term.app f x)) S⟫ →
@@ -49,9 +48,9 @@ notation P `⊢` e `:` Q : 10 := exp.vcgen P e Q
     f ∈ FV P →
     x ∈ FV P →
     y ∉ FV P →
-    (P && prop.call f x && (y ≡ term.app f x) && prop.post f x ⊢ e : Q) →
+    (P && prop.call f x && prop.post f x && (y ≡ term.app f x) ⊢ e : Q) →
     ⟪ prop.implies (P && prop.call f x) (term.unop unop.isFunc f && prop.pre f x) ⟫ →
-    (P ⊢ letapp y = f [x] in e : propctx.exis y (prop.call f x && (y ≡ term.app f x) && prop.post f x && Q))
+    (P ⊢ letapp y = f [x] in e : propctx.exis y (prop.call f x && prop.post f x && (y ≡ term.app f x) && Q))
 
 | ite {P: prop} {e₁ e₂: exp} {x: var} {Q₁ Q₂: propctx}:
     x ∈ FV P →
@@ -88,32 +87,34 @@ notation `⊢` σ `:` Q : 10 := env.vcgen σ Q
     (⊢ (σ[x ↦ value.num n]) : (Q && (x ≡ value.num n)))
 
 | func {σ₁ σ₂: env} {f g x: var} {R S: spec} {e: exp} {Q₁ Q₂: prop} {Q₃: propctx}:
-    f ∉ σ₁ →
+    g ∉ σ₁ →
     (⊢ σ₁ : Q₁) →
     (⊢ σ₂ : Q₂) →
-    FV R.to_prop ⊆ FV Q₂ ∪ { g, x } →
-    FV S.to_prop ⊆ FV Q₂ ∪ { g, x } →
-    (Q₂ && spec.func g x R S && R ⊢ e : Q₃) →
-    ⟪prop.implies (Q₂ && spec.func g x R S && R && Q₃ (term.app g x)) S⟫ →
-    (⊢ (σ₁[f ↦ value.func g x R S e σ₂]) : (Q₁ && (f ≡ value.func g x R S e σ₂)))
+    FV R.to_prop ⊆ FV Q₂ ∪ { f, x } →
+    FV S.to_prop ⊆ FV Q₂ ∪ { f, x } →
+    (Q₂ && spec.func f x R S && R ⊢ e : Q₃) →
+    ⟪prop.implies (Q₂ && spec.func f x R S && R && Q₃ (term.app f x)) S⟫ →
+    (⊢ (σ₁[g ↦ value.func f x R S e σ₂]) : (Q₁ && (g ≡ value.func f x R S e σ₂)))
 
 notation `⊢` σ `:` Q : 10 := env.vcgen σ Q
 
-inductive stack.vcgen : list call → stack → Prop
+inductive stack.vcgen : callhistory → stack → Prop
 notation H `⊩` s : 10 := stack.vcgen H s
 
-| top {H: list call} {P: prop} {σ: env} {e: exp} {Q: propctx}:
+| top {H: callhistory} {P: prop} {σ: env} {e: exp} {Q: propctx}:
     (⊢ σ : P) →
     (H && P ⊢ e : Q) →
     (H ⊩ (σ, e))
 
-| cons {H: list call} {P: prop} {s: stack} {σ σ': env} {f g x y z: var} {R S: spec} {e: exp} {v: value} {Q: propctx}:
+| cons {H: callhistory} {P: prop} {s: stack} {σ₁ σ₂: env} {f fx g x y: var} {R S: spec} {e: exp} {v: value} {Q: propctx}:
     (H ⊩ s) →
-    (⊢ σ : P) →
-    (σ f = value.func g z R S e σ') →
-    (σ x = v) →
-    ((σ[g↦value.func g z R S e σ'][z↦v], e) ⟶* s) →
-    (H && P ⊢ letapp y = f[x] in e : Q) →
-    (H ⊩ (s · [σ, let y = f[x] in e]))
+    (⊢ σ₁ : P) →
+    (σ₁ g = value.func f fx R S e σ₂) →
+    (σ₁ x = v) →
+    y ∉ σ₁ →
+    (H && P && prop.call g x && prop.post g x && (y ≡ term.app g x) ⊢ e : Q) →
+    ⟪ prop.implies (H && P && prop.call g x) (term.unop unop.isFunc g && prop.pre g x) ⟫ →
+    ((σ₂[f↦value.func f fx R S e σ₂][fx↦v], e) ⟶* s) →
+    (H ⊩ (s · [σ₁, let y = g[x] in e]))
 
 notation P `⊩` s : 10 := stack.vcgen P s
