freevars.lean
@@ -279,7 +279,7 @@ lemma free_in_vc.univ.same.inv {P: vc} {x: var}: ¬ free_in_vc x (vc.univ x P) :
     }
   end
 
-lemma call_history_closed (H: list call) (x: var): ¬ free_in_prop x (calls_to_prop H) :=
+lemma call_history_closed (H: callhistory) (x: var): ¬ free_in_prop x (calls_to_prop H) :=
   list.rec_on H
   ( -- empty history
     assume x_free: free_in_prop x (calls_to_prop list.nil),
@@ -292,103 +292,47 @@ lemma call_history_closed (H: list call) (x: var): ¬ free_in_prop x (calls_to_p
       }
     end
   )
-  ( -- <call> :: rest
-    assume ⟨f, x', R, S, e, σ, vₓ, v⟩,
-    assume rest: list call,
+  ( -- hist :: rest
+    assume h: historyitem,
+    assume rest: callhistory,
     assume ih: ¬ free_in_prop x (calls_to_prop rest),
-    assume x_free: free_in_prop x (calls_to_prop (⟨f, x', R, S, e, σ, vₓ, v⟩ :: rest)),
-    have calls_to_prop (⟨f, x', R, S, e, σ, vₓ, v⟩ :: rest) =
-      (prop.call (value.func f x' R S e σ) vₓ &&
-       prop.post (value.func f x' R S e σ) vₓ &&
-       (term.app (value.func f x' R S e σ) vₓ ≡ v) &&
-       calls_to_prop rest), from rfl,
-    have x_free_in_prop: free_in_prop x (
-      prop.call (value.func f x' R S e σ) vₓ &&
-      prop.post (value.func f x' R S e σ) vₓ &&
-      (term.app (value.func f x' R S e σ) vₓ ≡ v) &&
-      calls_to_prop rest), from this ▸ x_free,
-    have x_not_free_in_v: ¬ free_in_term x v, from (
-      assume x_free_in_v: free_in_term x v,
-      show «false», by cases x_free_in_v
-    ),
-    have x_not_free_in_vₓ: ¬ free_in_term x vₓ, from (
-      assume x_free_in_vₓ: free_in_term x vₓ,
-      show «false», by cases x_free_in_vₓ
-    ),
-    have x_not_free_in_f: ¬ free_in_term x (value.func f x' R S e σ), from (
-      assume x_free_in_f: free_in_term x (value.func f x' R S e σ),
-      show «false», by cases x_free_in_f
-    ),
-    have
-      free_in_prop x (calls_to_prop rest) ∨
-      free_in_prop x (prop.call (value.func f x' R S e σ) vₓ &&
-      prop.post (value.func f x' R S e σ) vₓ &&
-      (term.app (value.func f x' R S e σ) vₓ ≡ v)),
-    from (free_in_prop.and.inv x_free_in_prop).symm,
-    or.elim this ih (
-      assume x_free_in_call: free_in_prop x (
+    historyitem.cases_on h
+    ( -- <nop> :: rest
+      have h2: ¬ free_in_prop x (calls_to_prop rest), from ih,
+      have calls_to_prop (historyitem.nop :: rest) = calls_to_prop rest, by unfold calls_to_prop,
+      show ¬ free_in_prop x (historyitem.nop :: rest), from this.symm ▸ h2
+    )
+    ( -- <call> :: rest
+      assume f x' R S e σ vₓ,
+      assume x_free: free_in_prop x (calls_to_prop (call f x' R S e σ vₓ :: rest)),
+      have calls_to_prop (call f x' R S e σ vₓ :: rest) =
+        (prop.call (value.func f x' R S e σ) vₓ && calls_to_prop rest), by unfold calls_to_prop,
+      have x_free_in_prop: free_in_prop x (
         prop.call (value.func f x' R S e σ) vₓ &&
-        prop.post (value.func f x' R S e σ) vₓ &&
-        (term.app (value.func f x' R S e σ) vₓ ≡ v)),
+        calls_to_prop rest), from this ▸ x_free,
+      have x_not_free_in_vₓ: ¬ free_in_term x vₓ, from (
+        assume x_free_in_vₓ: free_in_term x vₓ,
+        show «false», by cases x_free_in_vₓ
+      ),
+      have x_not_free_in_f: ¬ free_in_term x (value.func f x' R S e σ), from (
+        assume x_free_in_f: free_in_term x (value.func f x' R S e σ),
+        show «false», by cases x_free_in_f
+      ),
       have
-        free_in_prop x (term.app (value.func f x' R S e σ) vₓ ≡ v) ∨
-        free_in_prop x (prop.call (value.func f x' R S e σ) vₓ &&
-          prop.post (value.func f x' R S e σ) vₓ),
-      from (free_in_prop.and.inv x_free_in_call).symm,
-      or.elim this (
-        assume x_free_in_eq_app: free_in_prop x (term.app (value.func f x' R S e σ) vₓ ≡ v),
+        free_in_prop x (calls_to_prop rest) ∨
+        free_in_prop x (prop.call (value.func f x' R S e σ) vₓ),
+      from (free_in_prop.and.inv x_free_in_prop).symm,
+      or.elim this ih (
+        assume x_free_in_call: free_in_prop x (prop.call (value.func f x' R S e σ) vₓ),
         show «false», by begin
-          cases x_free_in_eq_app,
-          case free_in_prop.term x_free_in_term {
-            cases x_free_in_term,
-            case free_in_term.binop₁ x_free_in_app {
-              cases x_free_in_app,
-              case free_in_term.app₁ x_free_in_f {
-                show «false», from x_not_free_in_f x_free_in_f
-              },
-              case free_in_term.app₂ x_free_in_vₓ {
-                show «false», from x_not_free_in_vₓ x_free_in_vₓ
-              }
-            },
-            case free_in_term.binop₂ x_free_in_v {
-              show «false», from x_not_free_in_v x_free_in_v
-            }
+          cases x_free_in_call,
+          case free_in_prop.call₁ x_free_in_f {
+            show «false», from x_not_free_in_f x_free_in_f
+          },
+          case free_in_prop.call₂ x_free_in_vₓ {
+            show «false», from x_not_free_in_vₓ x_free_in_vₓ
           }
         end
-      )
-      (
-        assume x_free_in_call_or_func: free_in_prop x (
-          prop.call (value.func f x' R S e σ) vₓ &&
-          prop.post (value.func f x' R S e σ) vₓ),
-        have
-          free_in_prop x (prop.call (value.func f x' R S e σ) vₓ) ∨
-          free_in_prop x (prop.post (value.func f x' R S e σ) vₓ),
-        from free_in_prop.and.inv x_free_in_call_or_func,
-        or.elim this
-        (
-          assume x_free_in_call: free_in_prop x (prop.call (value.func f x' R S e σ) vₓ),
-          show «false», by begin
-            cases x_free_in_call,
-            case free_in_prop.call₁ x_free_in_f {
-              show «false», from x_not_free_in_f x_free_in_f
-            },
-            case free_in_prop.call₂ x_free_in_vₓ {
-              show «false», from x_not_free_in_vₓ x_free_in_vₓ
-            }
-          end
-        )
-        (
-          assume x_free_in_post: free_in_prop x (prop.post (value.func f x' R S e σ) vₓ),
-          show «false», by begin
-            cases x_free_in_post,
-            case free_in_prop.post₁ x_free_in_f {
-              show «false», from x_not_free_in_f x_free_in_f
-            },
-            case free_in_prop.post₂ x_free_in_vₓ {
-              show «false», from x_not_free_in_vₓ x_free_in_vₓ
-            }
-          end
-        )
       )
     )
   )
