preservation.lean
@@ -1,5 +1,9 @@
 import .syntax .notations .logic .evaluation .vcgen
 
-theorem preservation {H: list call} {h: call} {s s': stack}:
-  (H ⊩ s) → (s ⟶ h, s') → (h :: H ⊩ s') ∧ ⟪[h]⟫
+lemma strengthen_pre_exp {P P': prop} {Q: propctx} {e: exp}:
+  (P ⊢ e : Q) → FV P' ⊆ FV P → (∀σ, σ ⊨ vc.implies P'.instantiated_n P.instantiated_n) → (P' ⊢ e: Q) :=
+  sorry
+
+theorem preservation {H: callhistory} {h: historyitem} {s s': stack}:
+  (H ⊩ s) → (s ⟶ h, s') → (h :: H ⊩ s')
 := sorry
