soundness.lean
@@ -1,17 +1,57 @@
+import data.set
+
 import .syntax .notations .logic .evaluation .vcgen .progress .preservation
 
-theorem soundness {e: exp} {s: stack}:
-  (list.nil ⊩ (env.empty, e)) → ((env.empty, e) ⟶* s) → (is_value s ∨ ∃s' h, s ⟶ h, s') :=
-  assume initial_verified: (list.nil ⊩ (env.empty, e)),
-  assume stepped_to_s: ((env.empty, e) ⟶* s),
-  begin
-    induction stepped_to_s,
-    case trans_step.rfl s_initial {
-      let H: list call := list.nil,
-      have H_valid: ⟪H⟫, from empty_history_valid,
-      show is_value s_initial ∨ ∃s' h, s_initial ⟶ h, s', from progress H H_valid initial_verified
-    },
-    case trans_step.trans a b c d e f {
+lemma trivial_precondition:
+  ∀σ, σ ⊨ vc.implies (prop.instantiated_n (value.true && value.true)) (prop.instantiated_n (value.true)) :=
+  assume σ: env,
+  show σ ⊨ vc.implies (prop.instantiated_n (value.true && value.true)) (prop.instantiated_n (value.true)),
+  from valid_env.mpr (
+    assume _,
+    have h: σ ⊨ value.true, from valid_env.true,
+    have prop.erased (prop.term value.true) = vc.term value.true, by unfold prop.erased,
+    have σ ⊨ (prop.erased (value.true)), from this.symm ▸ h,
+    have σ ⊨ (prop.instantiated (value.true)), from valid_env.instantiated_of_erased this,
+    show σ ⊨ (prop.instantiated_n (value.true)), from valid_env.instantiated_n_of_instantiated this
+  )
 
+lemma trivial_freevars: FV (prop.term value.true && prop.term value.true) ⊆ FV (prop.term value.true) :=
+  assume x: var,
+  assume : x ∈ FV (prop.term value.true && prop.term value.true),
+  have x ∈ FV (prop.term value.true) ∨ x ∈ FV (prop.term value.true), from free_in_prop.and.inv this,
+  or.elim this (
+    assume : x ∈ FV (prop.term value.true),
+    have x ∈ FV (term.value value.true), from free_in_prop.term.inv this,
+    show x ∈ FV (prop.term value.true), from absurd this free_in_term.value.inv
+  ) (
+    assume : x ∈ FV (prop.term value.true),
+    have x ∈ FV (term.value value.true), from free_in_prop.term.inv this,
+    show x ∈ FV (prop.term value.true), from absurd this free_in_term.value.inv
+  )
+
+lemma soundness {s s': stack}: (s ⟶* s') → ∀H, (H ⊩ s) → (is_value s' ∨ ∃h s'', s' ⟶ h, s'') :=
+  assume steps_to_s': s ⟶* s',
+  begin
+    induction steps_to_s',
+    case trans_step.rfl s₁ {
+      assume H,
+      assume s₁_verified ,
+      show is_value s₁ ∨ ∃h s', s₁ ⟶ h, s', from progress H s₁ s₁_verified
+    },
+    case trans_step.trans s₁ s₂ s₃ h s₁_steps_to_s₂ s₂_steps_to_s₃ ih {
+      assume H,
+      assume s₁_verified ,
+      have : (h :: H ⊩ s₂), from preservation s₁_verified s₁_steps_to_s₂,
+      show is_value s₃ ∨ ∃h s', s₃ ⟶ h, s', from ih (h::H) this
     }
   end
+
+theorem soundness_source_programs {e: exp} {s: stack} {Q: propctx}:
+  (value.true ⊢ e: Q) → ((env.empty, e) ⟶* s) → (is_value s ∨ ∃h s', s ⟶ h, s') :=
+
+  assume initial_verified: value.true ⊢ e: Q,
+  assume steps_to_s: (env.empty, e) ⟶* s,
+  have (prop.term value.true && prop.term value.true) ⊢ e: Q,
+  from strengthen_pre_exp initial_verified trivial_freevars trivial_precondition,
+  have list.nil ⊩ (env.empty, e), from stack.vcgen.top env.vcgen.empty this,
+  show is_value s ∨ ∃h s', s ⟶ h, s', from soundness steps_to_s list.nil this
